coq: Port proofs to accommodate arbitrary local optimizations

CircuitCorrectness.v
@@ -5,7 +5,8 @@ Import ListNotations.
 
 Require Import
         SGA.Common SGA.Environments SGA.Syntax
-        SGA.SemanticProperties SGA.CircuitProperties.
+        SGA.SemanticProperties SGA.CircuitProperties
+        SGA.CircuitElaboration SGA.Interop.
 
 Section CompilerCorrectness.
   Context {name_t var_t reg_t fn_t: Type}.
@@ -28,6 +29,7 @@ Section CompilerCorrectness.
   Context (sigma: forall f, ExternalSignature_denote (Sigma f)).
   Context (csigma: forall f, CExternalSignature_denote (cSigma f)).
   Context {csigma_correct: circuit_sigma_spec sigma csigma}.
+  Context (lco: local_circuit_optimizer cr csigma).
 
   Open Scope bool_scope.
 
@@ -178,19 +180,18 @@ Section CompilerCorrectness.
     intros cond * H0 H1 idx;
     unfold mux_rwsets; rewrite !getenv_map2;
     unfold mux_rwdata; cbn;
-    rewrite !opt1_correct; cbn;
+    rewrite !lco_proof; cbn;
     destruct (interp_circuit cond) as [ [ | ] [] ]; cbn;
     [ specialize (H1 eq_refl idx) | specialize (H0 eq_refl idx) ];
     eauto.
 
   Arguments EqDec_ListBool : simpl never.
-  Arguments opt1 : simpl never.
 
   Lemma log_data0_consistent'_mux :
     forall cond rws0 rws1 s l,
       (interp_circuit cond = Ob~0 -> log_data0_consistent' l rws0) ->
       (interp_circuit cond = Ob~1 -> log_data0_consistent' l rws1) ->
-      log_data0_consistent' l (mux_rwsets s cond rws1 rws0).
+      log_data0_consistent' l (mux_rwsets lco s cond rws1 rws0).
   Proof.
     log_consistent_mux_t.
   Qed.
@@ -200,6 +201,8 @@ Section CompilerCorrectness.
     eauto;
     let Heq := fresh in
     intros Heq; rewrite Heq in *; discriminate.
+
+  Notation mux_rwsets := (mux_rwsets lco).
 
   Lemma log_data0_consistent'_mux_l :
     forall cond rws0 rws1 s l,
@@ -333,6 +336,9 @@ Section CompilerCorrectness.
   Ltac ceauto :=
     eauto with circuits.
 
+  Notation willFire_of_canFire' := (willFire_of_canFire' lco).
+  Notation willFire_of_canFire := (willFire_of_canFire lco).
+
   Lemma interp_willFire_of_canFire_canFire_false :
     forall (c: circuit 1) (rwd: rwset) (cLog: scheduler_circuit R Sigma REnv),
       interp_circuit c = Ob~0 ->
@@ -360,7 +366,7 @@ Section CompilerCorrectness.
     induction finite_elements; cbn; intros.
     - bool_simpl; rewrite Bits.single_cons; reflexivity.
     - rewrite getenv_zip; cbn.
-      rewrite opt1_correct; cbn.
+      rewrite lco_proof; cbn.
       rewrite IHl; cbn.
       f_equal.
       rewrite <- !andb_assoc.
@@ -368,7 +374,7 @@ Section CompilerCorrectness.
       apply andb_comm.
   Qed.
 
-  Opaque willFire_of_canFire'.
+  Opaque Circuits.willFire_of_canFire'.
 
   Lemma finite_In {T} {FT: FiniteType T}:
     forall t: T, List.In t finite_elements.
@@ -430,7 +436,7 @@ Section CompilerCorrectness.
         eauto using @finite_In.
   Qed.
 
-  Transparent willFire_of_canFire'.
+  Transparent Circuits.willFire_of_canFire'.
 
   (* Lemma interp_willFire_of_canFire_willFire'_false : *)
   (*   forall clog (cLog: scheduler_circuit R Sigma REnv) idx, *)
@@ -514,6 +520,8 @@ Section CompilerCorrectness.
       eauto using rwset_circuit_lt_invariant_putenv_eq, rwset_circuit_lt_invariant_putenv_neq.
   Qed.
 
+  Notation mux_rwdata := (mux_rwdata lco).
+
   Lemma rwdata_circuit_lt_invariant_mux_rwdata_l :
     forall s c idx rwd1 rwd2 rwd3,
       (interp_circuit c = Ob~1 -> @rwdata_circuit_lt_invariant idx rwd1 rwd3) ->
@@ -533,6 +541,9 @@ Section CompilerCorrectness.
     unfold rwdata_circuit_lt_invariant, mux_rwdata; cbn; intros.
     repeat split; apply circuit_lt_CAnnot_r, circuit_lt_opt_r, circuit_lt_CMux_r; intuition eauto.
   Qed.
+
+  Notation compile_action := (compile_action lco).
+  Notation compile_scheduler := (compile_scheduler lco).
 
   Theorem rwset_circuit_lt_compile_action_correct {sig tau} :
     forall (gamma : ccontext sig) (a : action sig tau) (rwc : rwcircuit),
@@ -569,13 +580,13 @@ Section CompilerCorrectness.
         * apply circuit_lt_CAnnot_l, circuit_lt_opt_l, circuit_lt_CAnd_l, circuit_lt_refl.
         * intros. eapply rwset_circuit_lt_invariant_putenv.
           -- eauto using rwset_circuit_lt_invariant_refl.
-          -- red; cbn; eauto using circuit_lt_true, circuit_lt_refl.
+          -- red; cbn; eauto using circuit_lt_true, circuit_lt_refl, circuit_lt_opt_r.
       (* Read1 *)
       + split.
         * eauto using circuit_lt_refl.
         * intros; apply rwset_circuit_lt_invariant_putenv.
           -- eauto using rwset_circuit_lt_invariant_refl.
-          -- red; cbn; eauto using circuit_lt_true, circuit_lt_refl.
+          -- red; cbn; eauto using circuit_lt_true, circuit_lt_refl, circuit_lt_opt_r.
     - (* Write *)
       specialize (IHa gamma rwc) as (Hpr & Hpr').
       (* destruct port; cbn. *)
@@ -588,7 +599,7 @@ Section CompilerCorrectness.
             (apply rwset_circuit_lt_invariant_putenv;
              [ | specialize (Hpr' idx); red in Hpr' |- *; red in Hpr'; cbn;
                  repeat cleanup_step ];
-             intuition eauto using circuit_lt_true).
+             intuition eauto using circuit_lt_true, circuit_lt_opt_r).
     - (* Call *)
       specialize (IHa1 gamma rwc);
         specialize (IHa2 gamma (erwc (compile_action rc gamma a1 rwc))).
@@ -677,8 +688,8 @@ Section CompilerCorrectness.
     repeat match goal with
            | _ => progress intros
            | _ => reflexivity
-           | [ H: context[opt1] |- _ ] => rewrite opt1_correct in H
-           | [  |- context[opt1] ] => rewrite opt1_correct
+           | [ H: context[lco_fn] |- _ ] => rewrite lco_proof in H
+           | [  |- context[lco_fn] ] => rewrite lco_proof
            | _ => progress cbn
            | [ H: _ = _ |- _ ] => rewrite H
            | _ => destruct (Bits.single _)
@@ -687,8 +698,8 @@ Section CompilerCorrectness.
   Ltac t_interp_circuit_willFire_of_canFire_impl :=
     repeat match goal with
            | _ => reflexivity
-           | [ H: context[opt1] |- _ ] => rewrite opt1_correct in H
-           | [  |- context[opt1] ] => rewrite opt1_correct
+           | [ H: context[lco_fn] |- _ ] => rewrite lco_proof in H
+           | [  |- context[lco_fn] ] => rewrite lco_proof
            | _ => cleanup_step
            | _ => progress (unfold willFire_of_canFire'; cbn; intros)
            | [ H: Ob~_ = Ob~_ |- _ ] => apply (f_equal Bits.single) in H; cbn in H
@@ -849,7 +860,7 @@ Section CompilerCorrectness.
     t_interp_circuit_willFire_of_canFire_impl.
   Qed.
 
-  Arguments willFire_of_canFire' : simpl never.
+  Arguments Circuits.willFire_of_canFire' : simpl never.
 
   Lemma interp_circuit_willFire_of_canFire'_mux_rwdata:
     forall (idx : reg_t) s (rwd1 rwd2 : rwdata R Sigma (R idx)) (cCond : circuit 1) (rwdL : rwdata R Sigma (R idx)),
@@ -861,7 +872,7 @@ Section CompilerCorrectness.
   Proof.
     intros *;
       unfold willFire_of_canFire'; cbn.
-    repeat (rewrite !opt1_correct; cbn).
+    repeat (rewrite !lco_proof; cbn).
     destruct (interp_circuit cCond) as [ [ | ] [ ] ];
       cbn; eauto.
   Qed.
@@ -894,8 +905,8 @@ Section CompilerCorrectness.
     | _ => cleanup_step
     | _ => progress intros
     | _ => progress cbn in *
-    | [ H: context[opt1] |- _ ] => rewrite opt1_correct in H
-    | [  |- context[opt1] ] => rewrite opt1_correct
+    | [ H: context[lco_fn] |- _ ] => rewrite lco_proof in H
+    | [  |- context[lco_fn] ] => rewrite lco_proof
     | [ H: _ \/ _ |- _ ] => destruct H
     | [ H: exists _, _ |- _ ] => destruct H
     | [  |- Ob~_ = Ob~_ ] => f_equal
@@ -926,13 +937,15 @@ Section CompilerCorrectness.
   Ltac interp_willFire_cleanup :=
     repeat match goal with
            | _ => reflexivity
-           | [ H: interp_circuit (willFire_of_canFire _ _) = Ob~1 |- _ ] =>
+           (* The notations for willFire_of_canFire and willFire_of_canFire'
+              can't be used here, because of section variable (Coq bug?) *)
+           | [ H: interp_circuit (Circuits.willFire_of_canFire _ _ _) = Ob~1 |- _ ] =>
              rewrite interp_willFire_of_canFire_true in H
-           | [ H: interp_circuit (willFire_of_canFire _ _) = Ob~0 |- _ ] =>
+           | [ H: interp_circuit (Circuits.willFire_of_canFire _ _ _) = Ob~0 |- _ ] =>
              rewrite interp_willFire_of_canFire_false in H
-           | [ |- interp_circuit (willFire_of_canFire _ _) = Ob~1 ] =>
+           | [ |- interp_circuit (Circuits.willFire_of_canFire _ _ _) = Ob~1 ] =>
              rewrite interp_willFire_of_canFire_true
-           | [ |- interp_circuit (willFire_of_canFire _ _) = Ob~0 ] =>
+           | [ |- interp_circuit (Circuits.willFire_of_canFire _ _ _) = Ob~0 ] =>
              rewrite interp_willFire_of_canFire_false
            | _ => progress cbn
            | _ => progress intros
@@ -944,12 +957,12 @@ Section CompilerCorrectness.
              destruct (eq_dec idx idx'); subst;
              [ rewrite !get_put_eq | rewrite !get_put_neq by eassumption ];
              [ | solve [intuition eauto] ]
-           | [  |- interp_circuit (willFire_of_canFire' _ _) = Ob~_ ] =>
+           | [  |- interp_circuit (Circuits.willFire_of_canFire' _ _ _) = Ob~_ ] =>
              (rewrite interp_circuit_willFire_of_canFire_read0 ||
               rewrite interp_circuit_willFire_of_canFire_read1 ||
               rewrite interp_circuit_willFire_of_canFire_write0 ||
               rewrite interp_circuit_willFire_of_canFire_write1);
-             [ .. | solve[intuition eauto] ]
+             [ .. | solve[cbn; rewrite ?lco_proof; intuition eauto] ]
            | [ H: context[interp_circuit _ = _] |-
                context[interp_circuit _] ] =>
              rewrite H
@@ -959,7 +972,7 @@ Section CompilerCorrectness.
   Ltac may_read_write_t :=
     unfold may_read0, may_read1, may_write in *;
     repeat match goal with
-           | _ => rewrite opt1_correct in *
+           | _ => rewrite lco_proof in *
            | _ => progress bool_cleanup
            | [ H: log_rwdata_consistent _ ?regs |-
                context [Bits.single (interp_circuit (_ (REnv.(getenv) ?regs ?idx)))] ] =>
@@ -990,8 +1003,8 @@ Section CompilerCorrectness.
   Proof.
     induction ex; intros.
     - (* Fail *) t; interp_willFire_cleanup; t.
-    - (* Var *) cbn; rewrite opt1_correct; eauto.
-    - (* Const *) cbn; rewrite opt1_correct; eauto.
+    - (* Var *) cbn; rewrite lco_proof; eauto.
+    - (* Const *) cbn; rewrite lco_proof; eauto.
     - (* Seq *)
       t.
       eapply interp_circuit_circuit_lt_helper_false;
@@ -1042,9 +1055,9 @@ Section CompilerCorrectness.
       + cbn.
         destruct (may_read0 Log log idx) eqn:?; cbn.
         * repeat eapply conj.
-          -- rewrite opt1_correct; eauto.
+          -- rewrite lco_proof; eauto.
           -- apply log_rwdata_consistent_log_cons_putenv;
-               [ eauto | red ]; cbn; rewrite ?Bits.single_cons; eauto.
+               [ eauto | red ]; cbn; rewrite ?Bits.single_cons, lco_proof; eauto.
           -- apply log_data0_consistent_putenv_read_write1; eauto.
           -- apply log_data1_consistent_putenv_read_write0; eauto.
           -- interp_willFire_cleanup;
@@ -1063,7 +1076,7 @@ Section CompilerCorrectness.
         * repeat eapply conj.
           -- apply H1.
           -- apply log_rwdata_consistent_log_cons_putenv;
-               [ eauto | red ]; cbn; rewrite ?Bits.single_cons; eauto.
+               [ eauto | red ]; cbn; rewrite ?Bits.single_cons, lco_proof; eauto.
           -- apply log_data0_consistent_putenv_read_write1; eauto.
           -- apply log_data1_consistent_putenv_read_write0; eauto.
           -- interp_willFire_cleanup;
@@ -1076,21 +1089,21 @@ Section CompilerCorrectness.
     - (* Write *)
       t.
       + repeat apply conj.
-        * destruct port; reflexivity.
+        * destruct port;
+            interp_willFire_cleanup;
+            may_read_write_t.
         * destruct port;
             (apply log_rwdata_consistent_log_cons_putenv;
-             [ eauto | red ]; cbn; rewrite ?Bits.single_cons; eauto).
+             [ eauto | red ]; cbn; rewrite ?Bits.single_cons, lco_proof; eauto).
         * destruct port; cbn.
           -- apply log_data0_consistent_putenv_write0; eauto.
           -- apply log_data0_consistent_putenv_read_write1; eauto.
         * destruct port.
           -- apply log_data1_consistent_putenv_read_write0; eauto.
           -- apply log_data1_consistent_putenv_write1; eauto.
-        * destruct port.
-          -- interp_willFire_cleanup;
-               may_read_write_t.
-          -- interp_willFire_cleanup;
-               may_read_write_t.
+        * destruct port;
+            interp_willFire_cleanup;
+            may_read_write_t.
       + destruct port.
         * interp_willFire_cleanup;
             may_read_write_t; eauto.
@@ -1120,6 +1133,8 @@ Section CompilerCorrectness.
 
   Arguments update_accumulated_rwset : simpl never.
 
+  Notation update_accumulated_rwset := (update_accumulated_rwset lco).
+
   Lemma log_rwdata_consistent_update_accumulated_rwset:
     forall (l : Log) (l' : rwset) (L : Log) (L' : rwset),
       log_rwdata_consistent L L' ->
@@ -1129,7 +1144,7 @@ Section CompilerCorrectness.
     unfold log_rwdata_consistent, update_accumulated_rwset; intros * HL Hl ** ;
       rewrite getenv_map2; cbn.
     specialize (HL idx); specialize (Hl idx);
-      repeat (rewrite !opt1_correct || bool_cleanup || rewrite log_existsb_app);
+      repeat (rewrite !lco_proof || bool_cleanup || rewrite log_existsb_app);
       eauto.
   Qed.
 
@@ -1171,12 +1186,14 @@ Section CompilerCorrectness.
     red; intros; elim (mdestruct m).
   Qed.
 
+  Notation adapter := (adapter lco).
+
   Lemma log_rwdata_consistent_empty_adapter cLog:
     log_rwdata_consistent log_empty (regs (adapter cLog)).
   Proof.
     red; intros; cbn.
     rewrite getenv_map; cbn.
-    rewrite !log_existsb_empty; auto.
+    rewrite !log_existsb_empty, lco_proof; auto.
   Qed.
 
   Lemma log_data0_consistent_empty_adapter Log cLog:
@@ -1205,8 +1222,10 @@ Section CompilerCorrectness.
     interp_circuit (willFire_of_canFire (adapter cLog) cLog) = Ob~1.
   Proof.
     interp_willFire_cleanup.
-    rewrite getenv_map.
-    reflexivity.
+    - rewrite lco_proof; reflexivity.
+    - rewrite getenv_map.
+      unfold Circuits.willFire_of_canFire'.
+      t_interp_circuit_willFire_of_canFire.
   Qed.
 
   Hint Resolve circuit_gamma_equiv_empty : circuits.
@@ -1227,6 +1246,8 @@ Section CompilerCorrectness.
 
   Notation scheduler := (scheduler name_t).
   Context (rules: name_t -> rule).
+
+  Notation compile_scheduler' := (compile_scheduler' lco).
 
   Theorem scheduler_compiler'_correct':
     forall (s: scheduler) Log cLog,
@@ -1278,12 +1299,14 @@ Section CompilerCorrectness.
           apply IHs2; eauto.
   Qed.
 
+  Notation init_scheduler_circuit := (init_scheduler_circuit lco).
+
   Lemma log_rwdata_consistent_empty_init_scheduler:
     log_rwdata_consistent log_empty (init_scheduler_circuit rc).
   Proof.
     red; unfold init_scheduler_circuit, init_scheduler_rwdata;
       intros; rewrite !getenv_create, !log_existsb_empty; cbn;
-        eauto.
+        rewrite lco_proof; eauto.
   Qed.
 
   Lemma log_data0_consistent'_empty_init_scheduler:
@@ -1292,7 +1315,7 @@ Section CompilerCorrectness.
   Proof.
     red; unfold init_scheduler_circuit, init_scheduler_rwdata, circuit_env_equiv;
       intros; rewrite !getenv_create; cbn;
-        rewrite opt1_correct, latest_write0_empty; eauto.
+        rewrite lco_proof, latest_write0_empty; eauto.
   Qed.
 
   Lemma log_data1_consistent'_empty_init_scheduler:
@@ -1389,7 +1412,7 @@ Section CompilerCorrectness.
   Proof.
     intros; unfold compile_scheduler, commit_update, commit_rwdata, interp_scheduler.
     rewrite !getenv_map2, !getenv_create; cbn.
-    repeat (rewrite !opt1_correct; cbn).
+    repeat (rewrite !lco_proof; cbn).
     pose proof (scheduler_compiler'_correct' s log_empty (init_scheduler_circuit rc)
                                              ltac:(ceauto) ltac:(ceauto)
                                              ltac:(ceauto) ltac:(ceauto)) as (Hrv & Hcst0 & Hcst1).
@@ -1415,7 +1438,7 @@ Section CompilerCorrectness.
   Qed.
 End CompilerCorrectness.
 
-Section Thm.
+Section CircuitInit.
   Context {name_t var_t reg_t fn_t: Type}.
   Context {eq_dec_var_t: EqDec var_t}.
 
@@ -1436,34 +1459,56 @@ Section Thm.
       rewrite getenv_map; cbn;
         reflexivity.
   Qed.
+End CircuitInit.
 
-  Definition circuit_fn_of_fn {sig} (fn: ExternalSignature_denote sig)
-    : CExternalSignature_denote (CExternalSignature_of_ExternalSignature sig) :=
-    fun bs1 bs2 => bits_of_value (fn (value_of_bits bs1) (value_of_bits bs2)).
+Section Thm.
+  Context {name_t var_t reg_t fn_t: Type}.
+  Context {eq_dec_var_t: EqDec var_t}.
 
-  Definition circuit_sigma : forall f, CExternalSignature_denote (circuit_Sigma Sigma f) :=
-    fun f => circuit_fn_of_fn (sigma f).
+  Context {R: reg_t -> type}.
+  Context {Sigma: fn_t -> ExternalSignature}.
+  Context {REnv: Env reg_t}.
 
-  Lemma circuit_sigma_spec_bits_of_value :
-    circuit_sigma_spec sigma circuit_sigma.
-  Proof.
-    unfold circuit_sigma_spec, circuit_sigma, circuit_fn_of_fn.
-    intros; rewrite !value_of_bits_of_value.
-    reflexivity.
-  Qed.
+  Context (r: REnv.(env_t) R).
+  Context (sigma: forall f, Sigma f).
 
-  Context (rules: name_t -> rule var_t R Sigma).
   Context (s: scheduler name_t).
 
-  Theorem scheduler_compiler_correct:
-    let spec_results := commit_update r (interp_scheduler r sigma rules s) in
-    let circuits := compile_scheduler (REnv.(create) CReadRegister) rules s in
-    forall reg,
-      interp_circuit (circuit_r r) (circuit_sigma) (REnv.(getenv) circuits reg) =
-      bits_of_value (REnv.(getenv) spec_results reg).
-  Proof.
-    eauto using scheduler_compiler_correct',
+  Section Standalone.
+    Context (rules: name_t -> rule var_t R Sigma).
+
+    Theorem scheduler_compiler_correct:
+      forall (lco: local_circuit_optimizer (circuit_r r) (circuit_sigma sigma)),
+        let spec_results := commit_update r (interp_scheduler r sigma rules s) in
+        let circuits := compile_scheduler lco (REnv.(create) CReadRegister) rules s in
+        forall reg,
+          interp_circuit (circuit_r r) (circuit_sigma sigma) (REnv.(getenv) circuits reg) =
+          bits_of_value (REnv.(getenv) spec_results reg).
+    Proof.
+      eauto using scheduler_compiler_correct',
       circuit_env_equiv_CReadRegister,
-      circuit_sigma_spec_bits_of_value.
-  Qed.
+      circuit_sigma_spec_circuit_sigma.
+    Qed.
+  End Standalone.
+
+  Section Interop.
+    Context (rules: name_t -> rule var_t R (interop_Sigma Sigma)).
+
+    Definition interop_lco :=
+      lco_compose
+        (bool_simpl_lco (r := circuit_r r))
+        (external_elaboration_lco (Sigma := Sigma) (custom_sigma := sigma) (custom_fn_t := fn_t)).
+
+    Theorem scheduler_compiler_correct_interop:
+      let spec_results := commit_update r (interp_scheduler r (interop_sigma sigma) rules s) in
+      let circuits := compile_scheduler interop_lco (REnv.(create) CReadRegister) rules s in
+      forall reg,
+        interp_circuit (circuit_r r) (circuit_sigma (interop_sigma sigma)) (REnv.(getenv) circuits reg) =
+        bits_of_value (REnv.(getenv) spec_results reg).
+    Proof.
+      eauto using scheduler_compiler_correct',
+      circuit_env_equiv_CReadRegister,
+      circuit_sigma_spec_circuit_sigma.
+    Qed.
+  End Interop.
 End Thm.
